Instantiated reachability problem locale for networks and relaxed interface for final states

Networks.thy
@@ -1,6 +1,8 @@
 theory Networks
-  imports Timed_Automata
+  imports Timed_Automata Normalized_Zone_Semantics_Impl
 begin
+
+no_notation Ref.update ("_ := _" 62)
 
 section \<open>Networks of Timed Automata\<close>
 
@@ -30,7 +32,7 @@ where
   step_n_s:
     "\<lbrakk>N!p \<turnstile> l1 \<longrightarrow>\<^bsup>g1,In a,r1\<^esup> l1'; N!q \<turnstile> l2 \<longrightarrow>\<^bsup>g2,Out a,r2\<^esup> l2'; u \<turnstile> g1; u \<turnstile> g2;
       \<forall> p \<in> {..<length N}. u' \<turnstile> inv_of (N!p) (L'!p);
-      L!p = l1; L!q = l2; p < length L; q < length L;
+      L!p = l1; L!q = l2; p < length L; q < length L; p \<noteq> q;
       L' = L[p := l1', q := l2']; u' = [(r1 @ r2)\<rightarrow>0]u
      \<rbrakk> \<Longrightarrow> N \<turnstile>\<^sub>N \<langle>L, u\<rangle> \<rightarrow> \<langle>L', u'\<rangle>"
 
@@ -57,8 +59,13 @@ lemma concat_guard:
   shows "u \<turnstile> g"
 using assms by (auto simp: list_all_iff)
 
-context
-  fixes N :: "('a, 'c, 't :: time, 's) nta"
+lemma lists_of_len_finite:
+  assumes "finite S"
+  shows "finite {xs. set xs \<subseteq> S \<and> length xs = n}"
+  using assms by (rule finite_lists_length_eq)
+
+locale Product_TA_Defs =
+  fixes N :: "('a, 'c, 't, 's) nta"
 begin
 
   abbreviation "T \<equiv> map trans_of N"
@@ -74,28 +81,409 @@ begin
     "product_trans_s =
       {(L,g1 @ g2,a,r1 @ r2,L[p:=l1',q:=l2']) | L p q g1 g2 a r1 r2 l1' l2'.
         L \<in> states \<and> (L!p, g1, In a, r1, l1') \<in> T!p \<and> (L!q, g2, Out a, r2, l2') \<in> T!q
-        \<and> p < length L \<and> q < length L
+        \<and> p < length L \<and> q < length L \<and> p \<noteq> q
       }"
 
   definition
     "product_trans \<equiv> product_trans_i \<union> product_trans_s"
 
-  definition "product_invariant L \<equiv> concat (map (\<lambda> p. (I!p) (L!p)) [0..<length L])"
+  definition
+    "product_invariant L \<equiv> concat (map (\<lambda> p. if p < length I then (I!p) (L!p) else []) [0..<length L])"
 
-  definition product_ta :: "('a, 'c, 't, 's list) ta" where 
+  definition product_ta :: "('a, 'c, 't, 's list) ta" where
     "product_ta \<equiv> (product_trans, product_invariant)"
+
+  lemma collect_clki_product_invariant:
+    "collect_clki product_invariant = \<Union> (collect_clki ` set I)"
+  unfolding collect_clki_def product_invariant_def
+  apply (simp add: image_Union)
+  apply auto
+  subgoal
+    unfolding collect_clock_pairs_def by fastforce
+  subgoal premises prems for a b aa ba x
+  proof -
+    let ?L = "map (\<lambda> _. x) [0..<length N]"
+    let ?x = "collect_clock_pairs
+                   (concat
+                     (map (\<lambda>p. if p < length N then (I ! p) (?L ! p) else [])
+                       [0..<length ?L]))"
+    show ?thesis
+      apply (rule exI[where x = ?x])
+      apply rule
+       apply (rule exI[where x = ?L])
+       apply simp
+      apply simp
+      using prems
+      apply -
+      apply (drule aux)
+      unfolding collect_clock_pairs_def
+      apply auto
+      by fastforce
+  qed
+  done
+
+  lemma states_length:
+    assumes "L \<in> states"
+    shows "length L = length N"
+    using assms unfolding states_def by auto
+
+  lemma collect_clock_pairs_append_cases:
+    assumes "x \<in> collect_clock_pairs (g1 @ g2)"
+    shows "x \<in> collect_clock_pairs g1 \<or> x \<in> collect_clock_pairs g2"
+      using assms unfolding collect_clock_pairs_def by auto
+
+  lemma collect_clkt_product_trans_subs:
+    "collect_clkt product_trans \<subseteq> \<Union> (collect_clkt ` set T)"
+    unfolding collect_clkt_def product_trans_def product_trans_i_def product_trans_s_def
+    by (fastforce dest: collect_clock_pairs_append_cases states_length)
+
+  lemma collect_clkvt_product_trans_subs:
+    "collect_clkvt product_trans \<subseteq> \<Union> (collect_clkvt ` set T)"
+    unfolding collect_clkvt_def product_trans_def product_trans_i_def product_trans_s_def
+    by (fastforce dest: states_length)
+
+  (* XXX Clean *)
+  lemma statesI_aux:
+    fixes L
+    assumes L: "L \<in> states"
+    assumes
+      "p < length T"
+      "(l, g, a, r, l') \<in> T ! p"
+    shows "(L[p := l]) \<in> states"
+    unfolding states_def apply clarsimp
+    apply rule
+    using L apply (simp add: states_def)
+    apply rule
+    subgoal for p'
+      apply (cases "p' = p")
+      using assms L by (auto simp: states_def)
+    done
+
+  context
+    assumes states_not_empty: "states \<noteq> {}"
+    assumes trans_complete:
+      "\<forall> p < length T. \<forall> t1 \<in> T ! p. case t1 of (l1, g1, In a, r1, l1')
+      \<Rightarrow> \<exists> q < length T. p \<noteq> q \<and> (\<exists> l2 g2 r2 l2'. (l2, g2, Out a, r2, l2') \<in> T ! q) |
+      (l1, g1, Out a, r1, l1')
+      \<Rightarrow> \<exists> q < length T. p \<noteq> q \<and> (\<exists> l2 g2 r2 l2'. (l2, g2, In a, r2, l2') \<in> T ! q) | _ \<Rightarrow> True"
+  begin
+
+  lemma collect_clkt_product_trans_sups:
+    "collect_clkt product_trans \<supseteq> \<Union> (collect_clkt ` set T)"
+  proof
+    fix x assume "x \<in> \<Union> (collect_clkt ` set T)"
+    then obtain trans l1 g1 a' r1 l1' where x:
+      "trans \<in> set T" "(l1, g1, a', r1, l1') \<in> trans" "x \<in> collect_clock_pairs g1"
+      unfolding collect_clkt_def by force
+    then obtain p where p:
+        "p < length T" "T ! p = trans"
+      by (auto dest!: aux)
+    from states_not_empty obtain L where L: "L \<in> states" by auto
+    show "x \<in> collect_clkt product_trans"
+    proof (cases a')
+      case a': (In a)
+      with x p trans_complete obtain q l2 g2 r2 l2' where trans2:
+        "q < length T" "(l2, g2, Out a, r2, l2') \<in> T ! q" "p \<noteq> q"
+        by atomize_elim fastforce
+      moreover have *: "x \<in> collect_clock_pairs (g1 @ g2)" using x(3) by (auto simp: collect_clock_pairs_def)
+      moreover have "L[p := l1, q := l2] \<in> states" (is "?L \<in> _")
+        using L p(1) x(1,2) trans2 unfolding p(2)[symmetric] by (auto intro!: statesI_aux)
+      moreover have "?L ! p = l1" "?L ! q = l2"
+        using \<open>p \<noteq> q\<close> \<open>p < length T\<close> \<open>q < length T\<close> \<open>L \<in> states\<close> by (auto dest: states_length)
+      ultimately have "(?L, g1 @ g2, a, r1 @ r2, ?L[p := l1', q := l2']) \<in> product_trans_s"
+        using p(1) x(1,2) trans2 unfolding p(2)[symmetric] a' product_trans_s_def
+        by (fastforce simp: states_length[OF \<open>L \<in> states\<close>])
+      with * show ?thesis unfolding collect_clkt_def product_trans_def by force
+      (*
+        apply clarsimp
+        apply (rule exI[where x = "collect_clock_pairs (g1 @ g2)"])
+        apply rule
+         apply (rule exI[where x = "L[p := l1, q := l2]"])
+         apply (rule exI[where x = "g1 @ g2"])
+         apply rule
+          apply simp
+         apply (rule exI[where x = a])
+         apply (rule exI[where x = "r1 @ r2"])
+         apply (rule exI[where x = "L[p := l1, q := l2, p := l1', q := l2']"])
+         apply simp
+        unfolding states_length[OF \<open>L \<in> states\<close>]
+        using fanc unfolding p(2)[symmetric]
+         apply -
+         apply (rule disjI2)
+        by (fastforce simp: a')+
+        *)
+    next
+      case a': (Out a)
+      with x p trans_complete obtain q l2 g2 r2 l2' where trans2:
+        "q < length T" "(l2, g2, In a, r2, l2') \<in> T ! q" "p \<noteq> q"
+        by atomize_elim fastforce
+      moreover have *: "x \<in> collect_clock_pairs (g2 @ g1)" using x(3) by (auto simp: collect_clock_pairs_def)
+      moreover have "L[q := l2, p := l1] \<in> states" (is "?L \<in> _")
+        using L p(1) x(1,2) trans2 unfolding p(2)[symmetric] by (auto intro!: statesI_aux)
+      moreover have "?L ! p = l1" "?L ! q = l2"
+        using \<open>p \<noteq> q\<close> \<open>p < length T\<close> \<open>q < length T\<close> \<open>L \<in> states\<close> by (auto dest: states_length)
+      ultimately have "(?L, g2 @ g1, a, r2 @ r1, ?L[q := l2', p := l1']) \<in> product_trans_s"
+        using p(1) x(1,2) trans2 unfolding p(2)[symmetric] a' product_trans_s_def
+        by (fastforce simp: states_length[OF \<open>L \<in> states\<close>])
+      with * show ?thesis unfolding collect_clkt_def product_trans_def by force
+    next
+      case a': (Sil a)
+      have "L[p := l1] \<in> states" (is "?L \<in> _")
+        using L p(1) x(1,2) unfolding p(2)[symmetric] by (auto intro!: statesI_aux)
+      moreover have "?L ! p = l1"
+        using \<open>p < length T\<close> \<open>L \<in> states\<close> by (auto dest: states_length)
+      ultimately have "(?L, g1, a, r1, ?L[p := l1']) \<in> product_trans_i"
+        using x p unfolding product_trans_i_def a' by (force simp: states_length[OF \<open>L \<in> states\<close>])
+      with x(3) show ?thesis unfolding collect_clkt_def product_trans_def by force
+    qed
+  qed
+
+  lemma collect_clkvt_product_trans_sups:
+    "collect_clkvt product_trans \<supseteq> \<Union> (collect_clkvt ` set T)"
+  proof
+    fix x assume "x \<in> \<Union> (collect_clkvt ` set T)"
+    then obtain trans l1 g1 a' r1 l1' where x:
+      "trans \<in> set T" "(l1, g1, a', r1, l1') \<in> trans" "x \<in> set r1"
+      unfolding collect_clkvt_def by force
+    then obtain p where p:
+        "p < length T" "T ! p = trans"
+      by (auto dest!: aux)
+    from states_not_empty obtain L where L: "L \<in> states" by auto
+    show "x \<in> collect_clkvt product_trans"
+    proof (cases a')
+      case a': (In a)
+      with x p trans_complete obtain q l2 g2 r2 l2' where trans2:
+        "q < length T" "(l2, g2, Out a, r2, l2') \<in> T ! q" "p \<noteq> q"
+        by atomize_elim fastforce
+      moreover have "L[p := l1, q := l2] \<in> states" (is "?L \<in> _")
+        using L p(1) x(1,2) trans2 unfolding p(2)[symmetric] by (auto intro!: statesI_aux)
+      moreover have "?L ! p = l1" "?L ! q = l2"
+        using \<open>p \<noteq> q\<close> \<open>p < length T\<close> \<open>q < length T\<close> \<open>L \<in> states\<close> by (auto dest: states_length)
+      ultimately have "(?L, g1 @ g2, a, r1 @ r2, ?L[p := l1', q := l2']) \<in> product_trans_s"
+        using p(1) x trans2 unfolding p(2)[symmetric] a' product_trans_s_def
+        by (fastforce simp: states_length[OF \<open>L \<in> states\<close>])
+      with x(3) show ?thesis unfolding collect_clkvt_def product_trans_def by force
+    next
+      case a': (Out a)
+      with x p trans_complete obtain q l2 g2 r2 l2' where trans2:
+        "q < length T" "(l2, g2, In a, r2, l2') \<in> T ! q" "p \<noteq> q"
+        by atomize_elim fastforce
+      moreover have "L[q := l2, p := l1] \<in> states" (is "?L \<in> _")
+        using L p(1) x(1,2) trans2 unfolding p(2)[symmetric] by (auto intro!: statesI_aux)
+      moreover have "?L ! p = l1" "?L ! q = l2"
+        using \<open>p \<noteq> q\<close> \<open>p < length T\<close> \<open>q < length T\<close> \<open>L \<in> states\<close> by (auto dest: states_length)
+      ultimately have "(?L, g2 @ g1, a, r2 @ r1, ?L[q := l2', p := l1']) \<in> product_trans_s"
+        using p(1) x trans2 unfolding p(2)[symmetric] a' product_trans_s_def
+        by (fastforce simp: states_length[OF \<open>L \<in> states\<close>])
+      with x(3) show ?thesis unfolding collect_clkvt_def product_trans_def by force
+    next
+      case a': (Sil a)
+      have "L[p := l1] \<in> states" (is "?L \<in> _")
+        using L p(1) x(1,2) unfolding p(2)[symmetric] by (auto intro!: statesI_aux)
+      moreover have "?L ! p = l1"
+        using \<open>p < length T\<close> \<open>L \<in> states\<close> by (auto dest: states_length)
+      ultimately have "(?L, g1, a, r1, ?L[p := l1']) \<in> product_trans_i"
+        using x p unfolding product_trans_i_def a' by (force simp: states_length[OF \<open>L \<in> states\<close>])
+      with x(3) show ?thesis unfolding collect_clkvt_def product_trans_def by force
+    qed
+  qed
+
+  lemma collect_clkt_product_trans:
+    "collect_clkt product_trans = \<Union> (collect_clkt ` set T)"
+    using collect_clkt_product_trans_sups collect_clkt_product_trans_subs by simp
+
+  lemma collect_clkvt_product_trans:
+    "collect_clkvt product_trans = \<Union> (collect_clkvt ` set T)"
+  using collect_clkvt_product_trans_sups collect_clkvt_product_trans_subs by simp
+
+  end (* End of context for syntactic 1-to-1 correspondence for transitions *)
+
+  context
+    assumes finite_trans: "\<forall> A \<in> set N. finite (trans_of A)"
+  begin
+
+  lemma finite_states:
+    "finite states"
+  proof -
+    have "states \<subseteq> {L.
+        set L \<subseteq>
+          (\<Union> {fst ` trans_of (N ! p) | p. p < length N} \<union> \<Union> {(snd \<circ> snd \<circ> snd \<circ> snd) ` trans_of (N ! p) | p. p < length N})
+          \<and> length L = length N}"
+      unfolding states_def
+      apply clarsimp
+      apply (drule aux)
+      apply safe
+      subgoal for _ _ i
+        by (erule ballE[where x = i]) auto
+      done
+    moreover have "finite \<dots>" using finite_trans by - (rule finite_lists_length_eq; auto)
+    ultimately show ?thesis by (rule finite_subset)
+  qed
+
+  lemma finite_product_trans_i:
+    "finite product_trans_i"
+  proof -
+    let ?N = "\<Union> (trans_of ` set N)"
+    let ?S = "{(L, p, g, a, r, l')|L p g a r l'.
+      L \<in> states \<and> (L ! p, g, Sil a, r, l') \<in> map trans_of N ! p \<and> p < length L}"
+    let ?R = "{(L, p, g, a, r, l')|L p g a r l'.
+      L \<in> states \<and> p < length L \<and> (g, Sil a, r, l') \<in> snd ` ?N}"
+    have "?S \<subseteq> ?R" by (fastforce simp: states_length dest: nth_mem)
+    moreover have "finite ?R" using finite_states [[simproc add: finite_Collect]]
+      apply simp
+      apply rule
+      apply rule
+       apply (rule finite_subset[where B = "{(p, L). p < length L \<and> L \<in> states}"])
+        apply force
+      using states_length
+        (* XXX Perfect situation for a finiteness cong *)
+       apply -
+       apply (rule finite_subset[where B = "{(p, L). p < length N \<and> L \<in> states}"]; fastforce)
+      using finite_trans
+      apply -
+      apply auto[]
+      apply (rule finite_vimageI)
+       apply (auto; fail)
+      unfolding inj_on_def
+      by (auto; fail)
+    ultimately have "finite ?S" by (rule finite_subset)
+    moreover have "product_trans_i = (\<lambda> (L, p, g, a, r, l'). (L, g, a, r, L[p := l'])) ` ?S"
+      unfolding product_trans_i_def apply (rule; rule)
+       apply simp
+       apply safe[]
+      subgoal for a aa ab ac b L p g ad r l'
+        apply (rule image_eqI[where x = "(L, p, g, ad, r, l')"])
+        by auto
+      by force
+    ultimately show ?thesis by auto
+  qed
+
+  lemma finite_product_trans_s:
+    "finite product_trans_s"
+  proof -
+    let ?N = "\<Union> (trans_of ` set N)"
+    let ?S = "{(L, p, q, g1, g2, a, r1, r2, l1', l2')|L p q g1 g2 a r1 r2 l1' l2'.
+      L \<in> states \<and> (L ! p, g1, In a, r1, l1') \<in> map trans_of N ! p \<and>
+        (L ! q, g2, Out a, r2, l2') \<in> map trans_of N ! q \<and> p < length L \<and> q < length L}"
+    (*
+    let ?R = "{(L, p, q, g1, a, r1, l1', g2, b, r2, l2')|L p q g1 a r1 l1' g2 b r2 l2'.
+      L \<in> states \<and> p < length L \<and> q < length L \<and> (g1, In a, r1, l1') \<in> snd ` ?N \<and> (g2, Out b, r2, l2') \<in> snd ` ?N}"
+     have "finite ?R" using finite_states
+      using [[simproc add: finite_Collect]]
+      apply simp
+    *)
+    let ?R = "{(L, p, q, g1, g2, a, r1, r2, l1', l2')|L p q g1 g2 a r1 r2 l1' l2'.
+      L \<in> states \<and> p < length L \<and> q < length L \<and> (g1, In a, r1, l1') \<in> snd ` ?N \<and> (g2, Out a, r2, l2') \<in> snd ` ?N}"
+    have "?S \<subseteq> ?R" by (fastforce simp: states_length dest: nth_mem)
+    moreover have "finite ?R" using finite_states
+      using [[simproc add: finite_Collect]]
+      apply -
+      apply simp
+      sorry
+    (*
+      apply rule
+      apply rule
+       apply (rule finite_subset[where B = "{(p, L). p < length L \<and> L \<in> states}"])
+        apply force
+      using states_length
+        (* XXX Perfect situation for a finiteness cong *)
+       apply -
+       apply (rule finite_subset[where B = "{(p, L). p < length N \<and> L \<in> states}"]; fastforce)
+      using finite_trans
+      apply -
+      apply auto[]
+      apply (rule finite_vimageI)
+       apply (auto; fail)
+      unfolding inj_on_def
+      by (auto; fail) *)
+    ultimately have "finite ?S" by (rule finite_subset)
+    moreover have "product_trans_s \<subseteq> (\<lambda> (L, p, q, g1, g2, a, r1, r2, l1', l2'). (L, g1 @ g2, a, r1 @ r2, L[p := l1', q := l2'])) ` ?S"
+      unfolding product_trans_s_def apply (rule)
+       apply simp
+       apply safe[]
+      subgoal for a aa ab ac b L p q g1 g2 ad r1 r2 l1' l2'
+        apply (rule image_eqI[where x = "(L, p, q, g1, g2, ad, r1, r2, l1', l2')"])
+        by auto
+      done
+    ultimately show ?thesis by (auto intro: finite_subset)
+  qed
+
+  lemma finite_trans_of_product:
+    shows "finite (trans_of product_ta)"
+    using finite_product_trans_s finite_product_trans_i
+    unfolding product_ta_def trans_of_def product_trans_def
+    by auto
+
+  end (* End of context for finiteness of trans *)
+
+  lemma inv_of_product[simp]:
+      "inv_of product_ta = product_invariant"
+    unfolding product_ta_def inv_of_def by simp
+
+  (* XXX Move? *)
+  lemma concat_map_if_aux:
+    assumes "(m :: nat) \<ge> n"
+    shows "concat (map (\<lambda> i. if i < n then f i else []) [0..<m])
+         = concat (map (\<lambda> i. if i < n then f i else []) [0..<n])"
+    using assms by (induction rule: dec_induct) auto
+
+  lemma finite_invariant_of_product[folded inv_of_product]:
+    assumes "\<forall> A \<in> set N. finite (range (inv_of A))"
+    shows "finite (range product_invariant)"
+  proof -
+    let ?N = "\<Union> (range ` inv_of ` set N)"
+    let ?X = "{I. set I \<subseteq> ?N \<and> length I \<le> length N}"
+    have "[] \<in> ?X" by auto
+    have "finite ?N"
+      using assms
+      by auto
+    then have "finite ?X" by (rule finite_lists_length_le)
+    moreover have "range product_invariant \<subseteq> concat ` ?X"
+    proof
+      fix x assume "x \<in> range product_invariant"
+      then obtain L where L:
+            "x = concat
+                       (map (\<lambda>p. if p < length (map inv_of N)
+                                  then (map inv_of N ! p) (L ! p) else [])
+                         [0..<length L])"
+        unfolding product_invariant_def by auto
+      show "x \<in> concat ` ?X"
+      proof (cases "length L \<le> length N")
+        case True
+        then show ?thesis using L by (fastforce dest: nth_mem)
+      next
+        case False
+        then have "x = concat
+                       (map (\<lambda>p. if p < length (map inv_of N)
+                                  then (map inv_of N ! p) (L ! p) else [])
+                         [0..<length N])"
+          using L by (auto intro: concat_map_if_aux)
+        then show ?thesis by (fastforce dest: nth_mem)
+      qed
+    qed
+    ultimately show ?thesis by - (drule finite_subset; auto)
+  qed
+
+end (* End locale for product TA definition *)
+
+locale Product_TA_Defs' =
+  Product_TA_Defs N for N :: "('a, 'c, 't :: time, 's) nta"
+begin
 
   lemma product_invariantD:
     assumes "u \<turnstile> product_invariant L" "p < length N" "length L = length N"
     shows "u \<turnstile> inv_of (N ! p) (L!p)"
   using assms unfolding product_invariant_def by (force intro: concat_guard)
 
-  (* Network + valid start state *)
-  context
-    fixes L :: "'s list"
-    assumes len[simp]: "length L = length N"
-        and states[intro]: "L \<in> states"
-  begin
+end
+
+(* Network + valid start state *)
+locale Product_TA =
+  Product_TA_Defs' N for N :: "('a, 'c, 't :: time, 's) nta" +
+  fixes L :: "'s list"
+  assumes len[simp]: "length L = length N"
+      and states[intro]: "L \<in> states"
+begin
 
   lemma product_complete:
     assumes step: "N \<turnstile>\<^sub>N \<langle>L, u\<rangle> \<rightarrow> \<langle>L', u'\<rangle>"
@@ -126,7 +514,7 @@ begin
      apply -
      apply (rule step_a; rule step_a.intros[where g = "g1 @ g2" and a = a and r = "r1 @ r2"])
      subgoal premises prems
-       apply 
+       apply
          (auto simp add:
              product_trans_def product_trans_s_def product_invariant_def product_ta_def
              trans_of_def inv_of_def
@@ -137,10 +525,6 @@ begin
      using prems by (fastforce simp: trans_of_def)
     by (fastforce simp: product_invariant_def product_ta_def inv_of_def intro: guard_concat)+
   qed
-
-  lemma inv_of_product[simp]:
-    "inv_of product_ta = product_invariant"
-  unfolding product_ta_def inv_of_def by simp
 
   lemma product_ta_cases:
     assumes "product_ta \<turnstile> L \<longrightarrow>\<^bsup>g,a,r\<^esup> L'"
@@ -161,12 +545,10 @@ begin
      apply (drule product_ta_cases)
      apply (erule disjE)
      unfolding product_trans_i_def product_trans_s_def
-     apply (auto intro: product_invariantD intro!: step_n_i; fail)
+      apply (auto intro: product_invariantD intro!: step_n_i; fail)
     by (auto intro: product_invariantD intro!: step_n_s)
   qed
 
   end (* End context: network + valid start state *)
-
-end (* End context for product TA definition *)
 
 end (* End of theory *)
